Updating the definition to make them able to easily express invariants of the heap.

low/Invariants.v
@@ -13,98 +13,112 @@ Open Scope list_scope. (* FIXME: How to disable some notations of LibBag? *)
 
 (** ** A pointer is valid **)
 
-Definition bound (S : state) p := exists p_, read_SExp S p = Some p_.
+Definition bound_such_that (S : state) P p :=
+  exists p_, read_SExp S p = Some p_ /\ P p_.
+
+Definition bound S := bound_such_that S (fun _ => True).
+
+Lemma bound_such_that_weaken : forall S (P1 P2 : _ -> Prop) p,
+  (forall p_, P1 p_ -> P2 p_) ->
+  bound_such_that S P1 p ->
+  bound_such_that S P2 p.
+Proof. introv I (p_&E&H). exists* p_. Qed.
+
 
 (** ** Typed pointers **)
 
-Definition may_have_type (S : state) p l :=
-  exists p_, read_SExp S p = Some p_ /\ type p_ \in l.
+Definition may_have_types S l :=
+  bound_such_that S (fun p_ => type p_ \in l).
 
-Lemma may_have_type_bound : forall S p l,
-  may_have_type S p l ->
+Lemma may_have_types_bound : forall S p l,
+  may_have_types S l p ->
   bound S p.
-Proof. introv (p_&E&?). exists* p_. Qed.
+Proof. introv. apply* bound_such_that_weaken. Qed.
 
-Lemma may_have_type_nil : forall S p,
-  ~ may_have_type S p nil.
+Lemma may_have_types_nil : forall S p,
+  ~ may_have_types S nil p.
 Proof. introv (p_&E&M). applys~ BagInEmpty_list M. Qed.
 
-Lemma may_have_type_merge : forall S p l1 l2,
-  may_have_type S p l1 ->
-  may_have_type S p l2 ->
-  may_have_type S p (l1 \n l2).
+Lemma may_have_types_merge : forall S p l1 l2,
+  may_have_types S l1 p ->
+  may_have_types S l2 p ->
+  may_have_types S (l1 \n l2) p.
 Proof.
   introv (p1_&E1&M1) (p2_&E2&M2).
   rewrite E1 in E2. inverts E2. exists p2_. splits~.
   rewrite~ BagInter_list.
 Qed.
 
-Lemma may_have_type_weaken : forall S p l1 l2,
-  may_have_type S p l1 ->
+Lemma may_have_types_weaken : forall S p l1 l2,
+  may_have_types S l1 p ->
   l1 \c l2 ->
-  may_have_type S p l2.
-Proof. introv (p_&E&M) I. exists p_. splits~. applys~ BagInIncl M I. Qed.
+  may_have_types S l2 p.
+Proof. introv T I. applys~ bound_such_that_weaken T. introv M. applys~ BagInIncl M I. Qed.
 
 
 (** ** List pointers **)
 
-Definition list_type_step P (S : state) p l_t l_car l_tag : Prop :=
-  exists p_ header car cdr tag,
-    read_SExp S p = Some p_
-    /\ p_ = make_NonVector_SExpRec header (make_ListSxp_struct car cdr tag)
+Definition list_type_head P S l_t l_car l_tag (p_ : SExpRec) :=
+  exists header car cdr tag,
+    p_ = make_NonVector_SExpRec header (make_ListSxp_struct car cdr tag)
     /\ type p_ \in l_t
-    /\ may_have_type S car l_car
-    /\ P S cdr l_t l_car l_tag
-    /\ may_have_type S tag l_tag.
+    /\ may_have_types S l_car car
+    /\ P S l_t l_car l_tag cdr
+    /\ may_have_types S l_tag tag.
 
-Inductive list_type (S : state) : SEXP -> list SExpType -> list SExpType -> list SExpType -> Prop :=
+Definition list_type_step P (S : state) l_t l_car l_tag :=
+  bound_such_that S (list_type_head P S l_t l_car l_tag).
+
+Inductive list_type (S : state) : list SExpType -> list SExpType -> list SExpType -> SEXP -> Prop :=
   | list_type_nil : forall p l_t l_car l_tag,
-    may_have_type S p ([NilSxp]) ->
-    list_type S p l_t l_car l_tag
+    may_have_types S ([NilSxp]) p ->
+    list_type S l_t l_car l_tag p
   | list_type_cons : forall p l_t l_car l_tag,
-    list_type_step list_type S p l_t l_car l_tag ->
-    list_type S p l_t l_car l_tag
+    list_type_step list_type S l_t l_car l_tag p ->
+    list_type S l_t l_car l_tag p
   .
 
+Definition list_head := list_type_head list_type.
+
 Fixpoint list_type_ind' S
-    (P : SEXP -> list SExpType -> list SExpType -> list SExpType -> Prop)
+    (P : list SExpType -> list SExpType -> list SExpType -> SEXP -> Prop)
     (f_nil : forall p l_t l_car l_tag,
-       may_have_type S p ([NilSxp]) ->
-       P p l_t l_car l_tag)
+       may_have_types S ([NilSxp]) p ->
+       P l_t l_car l_tag p)
     (f_cons : forall p l_t l_car l_tag p_ header car cdr tag,
        read_SExp S p = Some p_ ->
        p_ = make_NonVector_SExpRec header (make_ListSxp_struct car cdr tag) ->
        type p_ \in l_t ->
-       may_have_type S car l_car ->
-       list_type S cdr l_t l_car l_tag ->
-       may_have_type S tag l_tag ->
-       P cdr l_t l_car l_tag ->
-       P p l_t l_car l_tag)
-    p l_t l_car l_tag (HL : list_type S p l_t l_car l_tag) : P p l_t l_car l_tag.
+       may_have_types S l_car car ->
+       list_type S l_t l_car l_tag cdr ->
+       may_have_types S l_tag tag ->
+       P l_t l_car l_tag cdr ->
+       P l_t l_car l_tag p)
+    l_t l_car l_tag p (HL : list_type S l_t l_car l_tag p) : P l_t l_car l_tag p.
   refine (
-    match HL in list_type _ p l_t l_car l_tag return P p l_t l_car l_tag with
+    match HL in list_type _ l_t l_car l_tag p return P l_t l_car l_tag p with
     | @list_type_nil _ p l_t l_car l_tag N =>
       f_nil p l_t l_car l_tag N
     | @list_type_cons _ p l_t l_car l_tag N => _
     end).
-  destruct N as (p_&h&car&cdr&tag&E&M&H&A&L&T).
+  destruct N as (p_&E&h&car&cdr&tag&M&H&A&L&T).
   refine (f_cons p l_t l_car l_tag _ _ _ _ _ E M H A L T _).
   applys~ list_type_ind' f_nil f_cons.
 Defined.
 
-Lemma list_type_may_have_type : forall S p l_t l_car l_tag,
-  list_type S p l_t l_car l_tag ->
-  may_have_type S p (l_t \u [NilSxp]).
+Lemma list_type_may_have_types : forall S p l_t l_car l_tag,
+  list_type S l_t l_car l_tag p ->
+  may_have_types S (l_t \u [NilSxp]) p.
 Proof.
-  introv I. destruct~ I as [? ? ? ? I|? ? ? ? (p_&h&car&cdr&tag&E&M&H&A&L&T)].
-  - applys may_have_type_weaken I. apply~ BagUnionIncl_right.
+  introv I. destruct~ I as [? ? ? ? I|? ? ? ? (p_&E&h&car&cdr&tag&M&H&A&L&T)].
+  - applys may_have_types_weaken I. apply~ BagUnionIncl_right.
   - exists p_. splits~. applys~ BagInIncl H. apply~ BagUnionIncl_left.
 Qed.
 
 Lemma list_type_merge : forall S p l1_t l2_t l1_car l2_car l1_tag l2_tag,
-  list_type S p l1_t l1_car l1_tag ->
-  list_type S p l2_t l2_car l2_tag ->
-  list_type S p (l1_t \n l2_t) (l1_car \n l2_car) (l1_tag \n l2_tag).
+  list_type S l1_t l1_car l1_tag p ->
+  list_type S l2_t l2_car l2_tag p ->
+  list_type S (l1_t \n l2_t) (l1_car \n l2_car) (l1_tag \n l2_tag) p.
 Proof.
   introv T1 T2. gen l2_t l2_car l2_tag.
   induction T1 as [? ? ? ? I1|? ? ? ? p1_ h1 car1 cdr1 tag1 E1 M1 H1 A1 L1 T1 IH]
@@ -112,30 +126,30 @@ Proof.
   - apply~ list_type_nil.
   - inverts T as T.
     + apply~ list_type_nil.
-    + inverts T as (h2&car2&cdr2&tag2&E2&M2&H2&A2&L2&T2).
+    + inverts T as (E2&h2&car2&cdr2&tag2&M2&H2&A2&L2&T2).
       rewrite E2 in E1. inversion E1 as [E1']. rewrite E1' in *.
       rewrite M1 in M2. inverts M2.
-      apply list_type_cons. exists p1_ h2 car2 cdr2 tag2. splits~.
+      apply list_type_cons. exists p1_. splits~. exists h2 car2 cdr2 tag2. splits~.
       * apply BagInter_list. splits~.
-      * applys~ may_have_type_merge A1 A2.
-      * applys~ may_have_type_merge T1 T2.
+      * applys~ may_have_types_merge A1 A2.
+      * applys~ may_have_types_merge T1 T2.
 Qed.
 
 Lemma list_type_weaken : forall S p l1_t l2_t l1_car l2_car l1_tag l2_tag,
   l1_t \c l2_t ->
   l1_car \c l2_car ->
   l1_tag \c l2_tag ->
-  list_type S p l1_t l1_car l1_tag ->
-  list_type S p l2_t l2_car l2_tag.
+  list_type S l1_t l1_car l1_tag p ->
+  list_type S l2_t l2_car l2_tag p.
 Proof.
   introv I1 I2 I3 T. gen l2_t l2_car l2_tag.
   induction T as [? ? ? ? I1|? ? ? ? p_ h car cdr tag E M H A L T IH]
     using list_type_ind'; introv Incl1 Incl2 Incl3.
   - apply~ list_type_nil.
-  - apply list_type_cons. exists p_ h car cdr tag. splits~.
+  - apply list_type_cons. exists p_. splits~. exists h car cdr tag. splits~.
     + applys~ BagInIncl H Incl1.
-    + applys~ may_have_type_weaken A Incl2.
-    + applys~ may_have_type_weaken T Incl3.
+    + applys~ may_have_types_weaken A Incl2.
+    + applys~ may_have_types_weaken T Incl3.
 Qed.
 
 
@@ -148,35 +162,32 @@ Record safe_SExpRec S (e_ : SExpRec) := make_safe_SExpRec {
       type e_ = NilSxp ->
       exists header car cdr tag,
         e_ = make_NonVector_SExpRec header (make_ListSxp_struct car cdr tag)
-        /\ may_have_type S car ([NilSxp])
-        /\ may_have_type S cdr ([NilSxp])
-        /\ may_have_type S tag ([NilSxp]) ;
+        /\ may_have_types S ([NilSxp]) car
+        /\ may_have_types S ([NilSxp]) cdr
+        /\ may_have_types S ([NilSxp]) tag ;
     SExpType_corresponds_to_data_SymSxp :
       type e_ = SymSxp ->
       exists header pname value internal,
         e_ = make_NonVector_SExpRec header (make_SymSxp_struct pname value internal)
-        /\ may_have_type S pname ([CharSxp])
-        (*/\ may_have_type S value ([(*TODO*)])
-        /\ may_have_type S internal ([(*TODO*)])*) ;
+        /\ may_have_types S ([CharSxp]) pname
+        (*/\ may_have_types S ([(*TODO*)]) value
+        /\ may_have_types S ([(*TODO*) internal])*) ;
     SExpType_corresponds_to_data_ListSxp :
       type e_ = ListSxp ->
-      exists header car cdr tag,
-        e_ = make_NonVector_SExpRec header (make_ListSxp_struct car cdr tag)
-        /\ may_have_type S cdr ([ListSxp])
-        /\ may_have_type S tag ([NilSxp ; CharSxp]) ;
+      list_head S ([ListSxp]) all_storable_SExpTypes ([NilSxp ; CharSxp]) e_ ;
     SExpType_corresponds_to_data_CloSxp :
       type e_ = CloSxp ->
       exists header formals body env,
         e_ = make_NonVector_SExpRec header (make_CloSxp_struct formals body env)
-        /\ may_have_type S formals ([NilSxp ; ListSxp])
-        (*/\ may_have_type S body ([(*TODO*)])*)
-        /\ may_have_type S env ([EnvSxp]) ;
+        /\ list_type S ([ListSxp]) all_storable_SExpTypes(*TODO*) ([NilSxp ; CharSxp]) formals
+        (*/\ may_have_types S ( body[(*TODO*)])*)
+        /\ may_have_types S ([EnvSxp]) env ;
     SExpType_corresponds_to_data_EnvSxp :
       type e_ = EnvSxp ->
       exists header frame enclos,
         e_ = make_NonVector_SExpRec header (make_EnvSxp_struct frame enclos)
-        /\ may_have_type S frame ([NilSxp ; ListSxp])
-        /\ may_have_type S enclos ([EnvSxp]) ;
+        /\ list_type S ([ListSxp]) all_storable_SExpTypes(*TODO*) ([NilSxp ; CharSxp]) frame
+        /\ may_have_types S ([EnvSxp]) enclos ;
     SExpType_corresponds_to_data_SpecialSxp :
       type e_ = SpecialSxp ->
       exists header offset,
@@ -217,14 +228,10 @@ Record safe_SExpRec S (e_ : SExpRec) := make_safe_SExpRec {
                (make_VecSxp_struct (ArrayList.length array) array))
         /\ forall a,
           Mem a (ArrayList.to_list array) ->
-          may_have_type S a ([CharSxp]) ;
+          may_have_types S ([CharSxp]) a ;
     SExpType_corresponds_to_data_DotSxp :
       type e_ = DotSxp ->
-      exists header car cdr tag,
-        e_ = make_NonVector_SExpRec header (make_ListSxp_struct car cdr tag)
-        (*/\ may_have_type S car ([(*TODO*)])*)
-        /\ may_have_type S cdr ([ListSxp])
-        /\ may_have_type S tag ([NilSxp]) ;
+      list_head S ([ListSxp ; DotSxp]) all_storable_SExpTypes ([NilSxp]) e_ ;
     SExpType_not_AnySxp :
       type e_ <> AnySxp ;
     SExpType_corresponds_to_data_VecSxp :
@@ -234,7 +241,7 @@ Record safe_SExpRec S (e_ : SExpRec) := make_safe_SExpRec {
                (make_VecSxp_struct (ArrayList.length array) array))
         (*/\ forall a,
           Mem a (ArrayList.to_list array) ->
-          may_have_type S a ([(*TODO*)])*) ;
+          may_have_types S ( a[(*TODO*)])*) ;
     SExpType_corresponds_to_data_ExprSxp :
       type e_ = ExprSxp ->
       exists header array,
@@ -242,7 +249,7 @@ Record safe_SExpRec S (e_ : SExpRec) := make_safe_SExpRec {
                (make_VecSxp_struct (ArrayList.length array) array))
         (*/\ forall a,
           Mem a (ArrayList.to_list array) ->
-          may_have_type S a ([(*TODO*)])*) ;
+          may_have_types S ( a[(*TODO*)])*) ;
     (** The following four types have not been implemented. **)
     SExpType_corresponds_to_data_BcodeSxp :
       type e_ = BcodeSxp -> True ;
@@ -284,7 +291,11 @@ Record safe_pointer S p := make_safe_pointer {
 Record safe_state S := make_safe_state {
     safe_entry_points : forall e p,
       move_along_entry_point e S = Some p ->
-      safe_pointer S p
+      safe_pointer S p ;
+    only_one_nil : forall p1 p2,
+      may_have_types S ([NilSxp]) p1 ->
+      may_have_types S ([NilSxp]) p2 ->
+      p1 = p2
   }.
 
 
@@ -337,10 +348,10 @@ Ltac simpl_list_inter :=
 
 Ltac simplify_context :=
   match goal with
-  | H1 : may_have_type ?S1 ?p1 ?l1,
-    H2 : may_have_type ?S2 ?p2 ?l2 |- _ =>
+  | H1 : may_have_types ?S1 ?l1 ?p1,
+    H2 : may_have_types ?S2 ?l2 ?p2 |- _ =>
     let H3 := fresh H1 H2 in
-    lets H3: may_have_type_merge (rm H1) (rm H2);
+    lets H3: may_have_types_merge (rm H1) (rm H2);
     rename H3 into H1
   | H1 : list_type ?S1 ?p1 ?l1_t ?l1_car ?l1_tag,
     H2 : list_type ?S2 ?p2 ?l2_t ?l2_car ?l2_tag |- _ =>
